WIP with fib

demo/fib/fib.c
@@ -1,0 +1,9 @@
+int fib(int n) {
+  if(n == 0)
+    return 0;
+  if(n == 1)
+    return 1;
+  int y1 = fib(n-2);
+  int y2 = fib(n-1);
+  return y1 + y2;
+}
