demo/fib/FibProof.v
@@ -1,0 +1,997 @@
+Require Import CoqlibC Maps Postorder.
+Require Import AST Linking.
+Require Import ValuesC MemoryC GlobalenvsC Events Smallstep.
+Require Import Op ClightC.
+Require Import CtypesC CtypingC.
+Require Import sflib.
+Require Import IntegersC.
+
+Require Import Simulation.
+Require Import Skeleton Mod ModSem SimMod SimModSemLift SimSymb SimMemLift MatchSimModSemExcl.
+Require SoundTop.
+Require SimMemId.
+Require Import Clightdefs.
+Require Import CtypesC.
+Require Import Any.
+Require Import SIRmini_quotient.
+Require Import FibSource.
+Require Import FibTarget.
+Require Import ModSemProps.
+Require Import Program.
+
+Set Implicit Arguments.
+
+Local Existing Instance SimMemOh_default.
+Local Arguments ModSemPair.mk [SM] [SS] _ _ _ _ [SMO].
+
+
+
+
+
+(********* TODO: try the same proof with extension ***************)
+(********* TODO: try the same proof with extension ***************)
+(********* TODO: try the same proof with extension ***************)
+(********* TODO: try the same proof with extension ***************)
+(********* TODO: try the same proof with extension ***************)
+(********* TODO: try the same proof with extension ***************)
+(********* TODO: try the same proof with extension ***************)
+(********* TODO: try the same proof with extension ***************)
+(********* TODO: try the same proof with extension ***************)
+(********* TODO: try the same proof with extension ***************)
+
+Lemma eq_eutt
+      E R
+      (a b: itree E R)
+      (EQ: a = b)
+  :
+    eutt eq a b
+.
+Proof. i. clarify. refl. Qed.
+
+Lemma vis_not_ret
+      E R (r: R) X (e: E X) k
+      (EUTT: Vis e k ≈ Ret r)
+  :
+    False
+.
+Proof. ii. punfold EUTT. inv EUTT. Qed.
+
+
+
+
+
+
+Section SIMMODSEM.
+
+Variable skenv_link: SkEnv.t.
+Variable sm_link: SimMem.t.
+Let md_src: Mod.t := (FibSource.module).
+Let md_tgt: Mod.t := (FibTarget.module).
+Hypothesis (INCLSRC: SkEnv.includes skenv_link (Mod.sk md_src)).
+Let INCLTGT: SkEnv.includes skenv_link (Mod.sk md_tgt).
+Proof. ss. Qed.
+Hypothesis (WF: SkEnv.wf skenv_link).
+Let ge := (SkEnv.project skenv_link (Mod.sk md_src)).
+Let tge := Build_genv (SkEnv.revive (SkEnv.project skenv_link (Mod.sk md_tgt)) prog) prog.(prog_comp_env).
+Definition msp: ModSemPair.t :=
+  ModSemPair.mk (md_src skenv_link) (md_tgt skenv_link) (SimSymbId.mk md_src md_tgt) sm_link.
+
+Let sk_same: __GUARD__ ((CSk.of_program signature_of_function FibTarget.prog) =
+                        (Sk.of_program (fn_sig (owned_heap:=owned_heap)) FibSource.prog)).
+Proof.
+  (*** TODO: generalize lemma and replace CshmgenproofC? ***)
+  unfold CSk.of_program, Sk.of_program. ss.
+Qed.
+
+Lemma unsymb
+      fid fblk
+      (FID: Genv.find_symbol ge fid = Some fblk)
+  :
+    <<FID: fid = _fib>>
+.
+Proof.
+  subst ge. ss. uge. ss. rewrite MapsC.PTree_filter_key_spec in *. des_ifs.
+  unfold defs in *. des_sumbool. ss. des; ss.
+  (*** TODO: strengthen "spec" !!!!!!!!!!! ***)
+  (*** TODO: strengthen "spec" !!!!!!!!!!! ***)
+  (*** TODO: strengthen "spec" !!!!!!!!!!! ***)
+  (* exploit (SkEnv.project_impl_spec); et. intro SPEC. *)
+  (* inv SPEC. *)
+  (* exploit (SYMBKEEP _iter); et. intro T. ss. folder. rewrite <- T in *. *)
+  (* exploit DEFKEEP; et. *)
+  (* assert(defs (md_src: Sk.t) _iter). *)
+  (* { ss. } *)
+  (* ss. *)
+Qed.
+
+Lemma symb
+  :
+    exists fblk, <<FID: Genv.find_symbol tge _fib = Some fblk>>
+.
+Proof.
+  Local Opaque _fib.
+  inv INCLSRC. ss.
+  exploit (DEFS _fib); et.
+  { unfold prog_defmap. ss. }
+  i; des. ss. rewrite sk_same. folder.
+  clear - SYMB.
+  subst ge. ss. uge. ss. rewrite MapsC.PTree_filter_key_spec. des_ifs. et.
+Qed.
+
+Lemma symb_def
+      fblk
+      (SYMB: Genv.find_symbol ge _fib = Some fblk)
+  :
+    <<DEF: Genv.find_funct tge (Vptr fblk Ptrofs.zero) = Some (Ctypes.Internal f_fib)>>
+.
+Proof.
+  exploit (SkEnv.project_impl_spec); try apply INCLSRC. intro SPECSRC.
+  exploit (SkEnv.project_impl_spec); try apply INCLTGT. intro SPECTGT.
+  des.
+  exploit SkEnv.project_revive_precise; et.
+  { unfold md_tgt in SPECTGT. ss. rewrite sk_same in *.
+    (* instantiate (1:= (SkEnv.project skenv_link *)
+    (*              (Sk.of_program (fn_sig (owned_heap:=owned_heap)) FibSource.prog))). *)
+    (* instantiate (3:= skenv_link). *)
+    (* instantiate (2:= (fn_sig (owned_heap:=owned_heap))). *)
+    (* instantiate (1:= FibSource.prog). *)
+    Fail eapply SPECTGT.
+    admit "universe".
+  }
+  { unfold md_tgt in INCLTGT. ss. rewrite sk_same in *. Fail eapply INCLTGT. admit "universe". }
+  i. inv H.
+  assert((prog_defmap FibTarget.prog) ! _fib = Some (Gfun (Internal f_fib))).
+  { ss. }
+  exploit P2GE; et.
+  { Fail eapply H.
+    admit "maybe universe". }
+  admit "giveup".
+Unshelve.
+  all: admit "giveup".
+Qed.
+
+
+
+
+
+Notation "'_'" := PTree.Leaf (at level 150).
+Notation "a % x % b" := (PTree.Node a x b) (at level 150).
+Notation "a %% b" := (PTree.Node a None b) (at level 150).
+
+Let te n: temp_env := (@PTree.Node val
+             (@PTree.Node val (@PTree.Leaf val) (@None val)
+                (@PTree.Node val
+                   (@PTree.Node val (@PTree.Leaf val) (@None val)
+                      (@PTree.Node val (@PTree.Leaf val) (@None val)
+                         (@PTree.Node val (@PTree.Leaf val) (@Some val Vundef) (@PTree.Leaf val))))
+                   (@None val)
+                   (@PTree.Node val
+                      (@PTree.Node val (@PTree.Leaf val) (@None val)
+                         (@PTree.Node val (@PTree.Leaf val) (@Some val Vundef) (@PTree.Leaf val)))
+                      (@None val) (@PTree.Leaf val)))) (@None val)
+             (@PTree.Node val
+                (@PTree.Node val (@PTree.Leaf val) (@None val)
+                   (@PTree.Node val
+                      (@PTree.Node val (@PTree.Leaf val) (@None val)
+                         (@PTree.Node val (@PTree.Leaf val) (@Some val (Vint n)) (@PTree.Leaf val)))
+                      (@None val) (@PTree.Leaf val))) (@None val)
+                (@PTree.Node val
+                   (@PTree.Node val (@PTree.Leaf val) (@None val)
+                      (@PTree.Node val (@PTree.Leaf val) (@None val)
+                         (@PTree.Node val (@PTree.Leaf val) (@Some val Vundef) (@PTree.Leaf val))))
+                   (@None val)
+                   (@PTree.Node val
+                      (@PTree.Node val (@PTree.Leaf val) (@None val)
+                         (@PTree.Node val (@PTree.Leaf val) (@Some val Vundef) (@PTree.Leaf val)))
+                      (@None val) (@PTree.Leaf val))))).
+
+Let k1 n k_tgt: cont :=
+  (Kcall (Some _t'1) f_fib empty_env (te n)
+          (Kseq (Sset _y1 (Etempvar _t'1 tint))
+             (Kseq
+                (Clight.Ssequence
+                   (Clight.Ssequence
+                      (Scall (Some _t'2)
+                         (Clight.Evar _fib (Tfunction (Tcons tint Tnil) tint cc_default))
+                         [Clight.Ebinop Cop.Osub (Etempvar _n tint) (Econst_int (Int.repr 2) tint)
+                            tint]) (Sset _y2 (Etempvar _t'2 tint)))
+                   (Clight.Sreturn
+                      (Some (Clight.Ebinop Cop.Oadd (Etempvar _y1 tint) (Etempvar _y2 tint) tint))))
+                k_tgt))).
+
+
+
+
+
+From ITree Require Export
+     KTree
+     KTreeFacts
+     Basics.CategoryOps
+     Basics.CategoryKleisli
+.
+
+(*** COPIED FROM MASTER BRANCH. REMOVE LATER ***)
+(*** COPIED FROM MASTER BRANCH. REMOVE LATER ***)
+(*** COPIED FROM MASTER BRANCH. REMOVE LATER ***)
+Lemma eutt_eq_bind : forall E R U (t1 t2: itree E U) (k1 k2: U -> itree E R), t1 ≈ t2 -> (forall u, k1 u ≈ k2 u) -> ITree.bind t1 k1 ≈ ITree.bind t2 k2.
+Proof.
+  intros.
+  eapply eutt_clo_bind with (UU := Logic.eq); [eauto |].
+  intros ? ? ->. apply H0.
+Qed.
+
+
+
+
+
+Import CatNotations.
+Open Scope cat_scope.
+Notation ktr := (ktree (EventE owned_heap) (owned_heap * (mem * val)) (owned_heap * (mem * val))).
+
+Definition is_call_cont_strong (k0: cont): Prop :=
+  match k0 with
+  | Kcall _ _ _ _ _ => True
+  | _ => False
+  end.
+
+Inductive match_stacks (n: int): ktr -> cont -> Prop :=
+| match_stacks_nil
+  :
+    match_stacks n (fun r => Ret r) Kstop
+| match_stacks_cons1
+    (hd_src tl_src: ktr)
+    (tl_tgt: cont)
+    (TL: match_stacks (Int.add n Int.one) tl_src tl_tgt)
+    (* n *)
+    (* (HDSRC: hd_src = *)
+    (*         (fun '(oh1, (m1, y1)) => *)
+    (*            '(oh2, (m2, y2)) <- trigger (ICall _sum oh1 m1 [Vint (Int.sub n (Int.repr 1))]) ;; *)
+    (*            Ret (oh2, (m2, Val.add y1 y2)))) *)
+    k_src k_tgt
+    (KSRC: k_src = (hd_src >>> tl_src))
+    (KTGT: k_tgt = k1 (Int.add n Int.one) tl_tgt)
+  :
+    match_stacks n k_src k_tgt
+(* | match_stacks_cons2 *)
+(*     (hd_src tl_src: ktr) *)
+(*     (tl_tgt: cont) *)
+(*     (TL: match_stacks (Int.add n (Int.repr 2)) tl_src tl_tgt) *)
+(*     k_src k_tgt *)
+(*     (KSRC: k_src = (hd_src >>> tl_src)) *)
+(*     (KTGT: k_tgt = k1 n tl_tgt) *)
+(*   : *)
+(*     match_stacks n k_src k_tgt *)
+.
+
+
+
+
+Inductive match_states_internal (i: nat): SIRmini_quotient.state owned_heap -> Clight.state ->
+                                          SimMem.t -> Prop :=
+| match_call
+    itr0 ty m0 vs n
+    fid fblk fptr_tgt k_src k_tgt
+    (VS: vs = [Vint n])
+    (* (ITR: itr0 ≈ interp_program0 IterSource.prog (ICall fid tt m0 vs)) *)
+    (STKS: match_stacks n k_src k_tgt)
+    (ITR: itr0 ≈ 'r <- (mrec (interp_function FibSource.prog) (ICall fid tt m0 vs)) ;; (k_src r))
+    (TY: ty = Clight.type_of_fundef (Internal f_fib))
+    (SYMB: Genv.find_symbol ge fid = Some fblk)
+    (FPTR: fptr_tgt = (Vptr fblk Ptrofs.zero))
+    (IDX: (i >= 100)%nat)
+  :
+    match_states_internal i (Eqv.lift itr0)
+                          (Clight.Callstate fptr_tgt ty vs k_tgt m0) (SimMemId.mk m0 m0)
+| match_return
+    itr0 m0 v k_src k_tgt n
+    (STKS: match_stacks n k_src k_tgt)
+    (RET: itr0 ≈ r <- Ret (tt, (m0, v)) ;; (k_src r))
+  :
+    match_states_internal i (Eqv.lift itr0) (Clight.Returnstate v k_tgt m0)
+                          (SimMemId.mk m0 m0)
+.
+
+Inductive match_states
+          (i: nat) (st_src0: state owned_heap) (st_tgt0: Clight.state) (smo0: SimMemOh.t): Prop :=
+| match_states_intro
+    (MATCHST: match_states_internal i st_src0 st_tgt0 smo0)
+    (MWF: SimMemOh.wf smo0)
+.
+
+Lemma bind_ret_map {E R1 R2} (u : itree E R1) (f : R1 -> R2) :
+  (r <- u ;; Ret (f r)) ≅ f <$> u.
+Proof.
+  rewrite <- (bind_ret_r u) at 2. apply eqit_bind.
+  - hnf. intros. apply eqit_Ret. auto.
+  - rewrite bind_ret_r. reflexivity.
+Qed.
+
+Lemma map_vis {E R1 R2 X} (e: E X) (k: X -> itree E R1) (f: R1 -> R2) :
+  (* (f <$> (Vis e k)) ≅ Vis e (fun x => f <$> (k x)). *)
+  ITree.map f (Vis e k) ≅ Vis e (fun x => f <$> (k x)).
+Proof.
+  cbn.
+  unfold ITree.map.
+  autorewrite with itree. refl.
+Qed.
+
+
+
+
+
+
+(*** TODO: IDK why but (1) ?UNUSNED is needed (2) "fold" tactic does not work. WHY????? ***)
+Ltac fold_eutt :=
+  repeat multimatch goal with
+         | [ H: eqit eq true true ?A ?B |- ?UNUSED ] =>
+           let name := fresh "tmp" in
+           assert(tmp: eutt eq A B) by apply H; clear H; rename tmp into H
+         end
+.
+
+Ltac des_itr itr :=
+  let name := fresh "V" in
+  destruct (observe itr) eqn:name; sym in name; eapply simpobs in name;
+  eapply bisimulation_is_eq in name; subst itr
+.
+
+Ltac vvt H := clear - H; exfalso; punfold H; inv H; simpl_depind; subst; simpl_depind.
+Ltac f_equiv := first [eapply eutt_eq_bind|eapply eqit_VisF|eapply eqit_bind'|Morphisms.f_equiv].
+
+Hint Rewrite @bind_trigger : itree.
+Hint Rewrite @tau_eutt : itree.
+Tactic Notation "irw" "in" ident(H) := repeat (autorewrite with itree in H; cbn in H).
+Tactic Notation "irw" := repeat (autorewrite with itree; cbn).
+
+
+
+
+
+
+
+
+Lemma init_fsim
+      args st_src0
+      (INIT: ModSem.initial_frame (md_src skenv_link) tt args st_src0)
+  :
+    exists i st_tgt0 smo0,
+      (<<INIT: ModSem.initial_frame (md_tgt skenv_link) tt args st_tgt0>>)
+      /\ (<<MATCH: match_states i st_src0 st_tgt0 smo0>>)
+.
+Proof.
+  inv INIT. ss. des_ifs. folder.
+  unfold interp_program0 in *.
+  exploit unsymb; et. i; des. clarify.
+  assert(SIG: fd = signature_of_function f_fib).
+  { admit "ez - findf sig". }
+  clarify. destruct args; ss. inv TYP. ss. destruct vs; ss. destruct vs; ss.
+  inv DEF. clear H2. unfold typify_list, typify in *; ss. des_ifs. destruct v; ss.
+  revert sk_same. revert INCLTGT. clear_tac. i.
+  eexists _, _, (SimMemId.mk _ _). esplits; eauto.
+  - econs; ss; eauto.
+    { rewrite sk_same. folder. exploit symb_def; et. }
+    { ss. }
+  - econs; ss; eauto. econs; ss; eauto.
+    + unfold typify_list. ss. unfold typify. des_ifs; ss.
+    + econs; ss.
+    + cbn. irw. rewrite ITR. unfold typify. des_ifs; ss. refl.
+Qed.
+
+(* Lemma final_fsim *)
+(*       i st_src0 st_tgt0 smo0 retv *)
+(*       (MATCH: match_states i st_src0 st_tgt0 smo0) *)
+(*       (FIN: ModSem.final_frame (md_src skenv_link) st_src0 tt retv) *)
+(*   : *)
+(*     exists smo_ret, *)
+(*       (<<FIN: ModSem.final_frame (md_tgt skenv_link)  st_tgt0 tt retv>>) /\ *)
+(*       (<<SIMRET: SimMem.sim_retv retv retv smo_ret>>) /\ *)
+(*       (<<MWF: SimMem.wf smo_ret>>) *)
+(* . *)
+(* Proof. *)
+(*   inv FIN. ss. *)
+(*   inv MATCH. ss. inv MATCHST; ss. *)
+(*   { rewrite RET in *. rewrite ITR in *. clear - IN. exfalso. *)
+(*     rewrite mrec_as_interp in IN. irw in IN. des_ifs; vvt IN. } *)
+(*   eexists (SimMemId.mk m0 m0). *)
+(*   esplits; ss; eauto; cycle 1. *)
+(*   { econs; eauto. ss. } *)
+(*   inv STKS; cycle 1. *)
+(*   { rewrite RET in *. rewrite RET0 in *. clear - IN. exfalso. *)
+(*     vvt IN. *)
+(* Qed. *)
+
+Lemma match_states_lxsim
+      idx st_src0 st_tgt0 sm0
+      (MATCH: match_states idx st_src0 st_tgt0 sm0)
+  :
+    <<XSIM: lxsimL (md_src skenv_link) (md_tgt skenv_link)
+                   (fun st => unit -> exists su m_init, SoundTop.sound_state su m_init st)
+                   top3 (fun _ _ => SimMemOh.le)
+                   (Ord.lift_idx lt_wf idx) st_src0 st_tgt0 sm0>>
+.
+Proof.
+  revert_until idx. revert idx.
+  pcofix CIH.
+  i.
+  pfold.
+  inv MATCH. subst; ss. ii. clear SUSTAR. inv MATCHST; ss; clarify.
+  - econs 1; eauto. ii. clear SU.
+    exploit unsymb; et. intro T. des; clarify.
+    exploit symb_def; et. intro DEF; des. ss. des_ifs.
+
+    rename ITR into V.
+    unfold interp_program0 in V. rewrite sk_same in *. folder.
+    rewrite mrec_as_interp in V. cbn in V. des_ifs. cbn in V.
+    (* unfold c_iter in V. *)
+
+
+    econs 1; et; swap 2 3.
+    { esplits; intro T; rr in T; des; inv T; ss; rewrite V in *; ss.
+      - rewrite VIS in IN. irw in IN. vvt IN.
+      - rewrite RET in IN. irw in IN. vvt IN.
+    }
+    { eapply modsem_receptive; et. }
+    ii. ss. inv STEPSRC; ss; rewrite V in IN; swap 3 4.
+    { rewrite VIS in IN. irw in IN. vvt IN. }
+    { rewrite VIS in IN. irw in IN. vvt IN. }
+    { rewrite VIS in IN. irw in IN. vvt IN. }
+    rewrite VIS in IN. autorewrite with itree in IN. cbn in IN. rewrite bind_trigger in IN.
+    apply eqit_inv_vis in IN. des. specialize (IN0 tt). fold_eutt.
+    rename k into itr2.
+
+    eexists _, _, (SimMemId.mk _ _). esplits; eauto.
+    { right. esplits; try apply star_refl.
+      apply Ord.lift_idx_spec. instantiate (1 := Nat.pred idx). xomega. }
+    left. pfold.
+
+    econs 1; et. intro T. revert sk_same. clear_tac. clear SUSTAR. i.
+    sym in IN0. unfold c_fib in IN0. unfold unwrapU in IN0.
+    clears itr0. clear itr0.
+    clears itr1. clear itr1.
+    rename IN0 into V.
+    (* destruct (classic (exists n, vs = [Vint n])); cycle 1. *)
+    (* { assert(UB: exists k, itr2 () ≈ Vis (EUB _) k). *)
+    (*   { des_ifs; try (unfold triggerUB in V; irw in V; eauto); *)
+    (*       try (by contradict H; esplits; et). *)
+    (*   } *)
+    (*   des. *)
+    (*   econs 1; et; swap 2 3. *)
+    (*   { esplits; intro T; rr in T; des; inv T; ss; rewrite V in *; ss. *)
+    (*     - rewrite VIS in IN. rewrite UB in IN. irw in IN. vvt IN. *)
+    (*     - rewrite RET in IN. rewrite UB in IN. irw in IN. vvt IN. *)
+    (*   } *)
+    (*   { eapply modsem_receptive; et. } *)
+    (*   ii. ss. inv STEPSRC; ss. *)
+    (*   - rewrite VIS in IN. rewrite UB in IN. irw in IN. vvt IN. *)
+    (*   - rewrite VIS in IN. rewrite UB in IN. irw in IN. vvt IN. *)
+    (*   - rewrite VIS in IN. rewrite UB in IN. irw in IN. vvt IN. *)
+    (*   - rewrite VIS in IN. rewrite UB in IN. irw in IN. vvt IN. *)
+    (* } *)
+    des. clarify. ss. irw in V. des_ifs_safe.
+    des_ifs.
+    { apply_all_once Int.same_if_eq. subst.
+      irw in V.
+      econs 2; try refl; eauto.
+      { esplits; eauto; cycle 1.
+        { apply Ord.lift_idx_spec. instantiate (1 := Nat.pred (Nat.pred idx)). xomega. }
+        eapply spread_dplus; et.
+        { eapply modsem2_mi_determinate; et. }
+        eapply plus_left with (t1 := E0) (t2 := E0); ss.
+        { repeat (econs; ss; et); ii; repeat (des; ss; clarify). }
+        eapply star_left with (t1 := E0) (t2 := E0); ss.
+        { repeat (econs; ss; et). }
+        eapply star_left with (t1 := E0) (t2 := E0); ss.
+        { repeat (econs; ss; et). }
+        eapply star_left with (t1 := E0) (t2 := E0); ss.
+        { repeat (econs; ss; et). }
+        eapply star_refl.
+      }
+      right. eapply CIH. econs; eauto.
+      - ss. econs; eauto; cycle 1.
+        { rewrite V. instantiate (1:= k_src). irw. refl. }
+        { inv STKS.
+          - econs; eauto.
+          - econs; eauto. }
+      - ss.
+    }
+    { apply_all_once Int.same_if_eq. subst.
+      irw in V.
+      econs 2; try refl; eauto.
+      { esplits; eauto; cycle 1.
+        { apply Ord.lift_idx_spec. instantiate (1 := Nat.pred (Nat.pred idx)). xomega. }
+        eapply spread_dplus; et.
+        { eapply modsem2_mi_determinate; et. }
+        eapply plus_left with (t1 := E0) (t2 := E0); ss.
+        { repeat (econs; ss; et); ii; repeat (des; ss; clarify). }
+        eapply star_left with (t1 := E0) (t2 := E0); ss.
+        { repeat (econs; ss; et). }
+        eapply star_left with (t1 := E0) (t2 := E0); ss.
+        { repeat (econs; ss; et). }
+        eapply star_left with (t1 := E0) (t2 := E0); ss.
+        { repeat (econs; ss; et). }
+        eapply star_left with (t1 := E0) (t2 := E0); ss.
+        { repeat (econs; ss; et). }
+        eapply star_left with (t1 := E0) (t2 := E0); ss.
+        { repeat (econs; ss; et). }
+        eapply star_left with (t1 := E0) (t2 := E0); ss.
+        { repeat (econs; ss; et). }
+        eapply star_refl.
+      }
+      right. eapply CIH. econs; eauto.
+      - ss. econs; eauto; cycle 1.
+        { rewrite V. instantiate (1:= k_src). irw. refl. }
+        { inv STKS.
+          - econs; eauto.
+          - econs; eauto. }
+      - ss.
+    }
+    { irw in V. rewrite mrec_as_interp in V. irw in V. des_ifs.
+      unfold triggerNB in *.
+      econs 2; try refl; eauto.
+      { esplits; eauto; cycle 1.
+        { apply Ord.lift_idx_spec. instantiate (1 := Nat.pred (Nat.pred idx)). xomega. }
+        eapply spread_dplus; et.
+        { eapply modsem2_mi_determinate; et. }
+        eapply plus_left with (t1 := E0) (t2 := E0); ss.
+        { repeat (econs; ss; et); ii; repeat (des; ss; clarify). }
+        eapply star_left with (t1 := E0) (t2 := E0); ss.
+        { repeat (econs; ss; et); ii; repeat (des; ss; clarify). }
+        eapply star_left with (t1 := E0) (t2 := E0); ss.
+        { repeat (econs; ss; et); ii; repeat (des; ss; clarify).
+          fold Int.zero. rewrite Heq. ss.
+        }
+        eapply star_left with (t1 := E0) (t2 := E0); ss.
+        { repeat (econs; ss; et); ii; repeat (des; ss; clarify). }
+        eapply star_left with (t1 := E0) (t2 := E0); ss.
+        { repeat (econs; ss; et); ii; repeat (des; ss; clarify). }
+        eapply star_left with (t1 := E0) (t2 := E0); ss.
+        { repeat (econs; ss; et); ii; repeat (des; ss; clarify).
+          fold Int.one. rewrite Heq0. ss. }
+        eapply star_left with (t1 := E0) (t2 := E0); ss.
+        { repeat (econs; ss; et); ii; repeat (des; ss; clarify). }
+        eapply star_left with (t1 := E0) (t2 := E0); ss.
+        { repeat (econs; ss; et); ii; repeat (des; ss; clarify). }
+        eapply star_left with (t1 := E0) (t2 := E0); ss.
+        { repeat (econs; ss; et); ii; repeat (des; ss; clarify). }
+        eapply star_left with (t1 := E0) (t2 := E0); ss.
+        { econsr; ss; et.
+          - econsr; ss; et.
+            + econsr; ss; et.
+            + econs 2; ss; et.
+          - repeat (econs; ss; et); ii; repeat (des; ss; clarify). }
+        apply star_refl.
+      }
+      fold (te n). right. eapply CIH.
+      econs; ss.
+      econs; ss; eauto.
+      - unfold Cop.cast_int_int.
+        assert(L: Int.add (Int.sub n (Int.repr 1)) Int.one = n).
+        { rewrite Int.sub_add_opp.
+          rewrite Int.add_assoc. rewrite Int.neg_repr.
+          unfold Int.one. rewrite Int.Ptrofs_add_repr. simpl.
+          rewrite Int.add_zero. eauto.
+        }
+        econs; eauto; try refl.
+        * rewrite L. eauto.
+        * unfold k1. repeat f_equal. rewrite L. eauto.
+      - rewrite V. f_equiv.
+        { rewrite mrec_as_interp.
+          f_equiv. irw. des_ifs_safe. cbn. rewrite <- bind_trigger.
+          f_equiv; try refl. admit "".
+        }
+        eapply eutt_eq_bind.  eutt_eq_bind. eqit_bind'. admit "".
+      - admit "idx".
+      - ss.
+    }
+  - econs 3; eauto.
+    { rr. esplits; et. econs; et.
+      - refl.
+      - admit "change is_call to NSTEP NRET".
+      - admit "change is_call to NSTEP NRET -- or put in match_states && exploit 'safe'". }
+    ii. ss. inv ATSRC. ss.
+    rewrite ITR in *. rewrite VIS in *. eapply eqit_inv_vis in IN. des. clarify.
+    eexists _, _, (SimMemId.mk _ _). ss. esplits; et.
+    { rr. ss. esplits; et. econs; ss; et. }
+    { econs; ss; et.
+      - rewrite sk_same. folder. admit "ez - FINDF".
+      - esplits; et. unfold sg in *. rewrite H4. unfold signature_of_type in *.
+        unfold Sk.get_sig in *. des_ifs. ss. rewrite <- H4. ss. }
+    ii.
+    inv AFTERSRC. inv GETK. ss.
+    rewrite ITR in *. rewrite VIS0 in *.
+    apply eqit_inv_vis in IN. des. clarify.
+    rr in SIMRETV. des. ss. clarify. revert sk_same. clear_tac. i. (*** TODO: update claer_tac ***)
+    inv SIMRETV0; ss. clarify.
+    unfold Retv.mk in *. clarify. destruct sm_ret ;ss. clarify.
+    rename tgt into m0. rename v_tgt into rv.
+    specialize (IN1 (tt, (m0, rv))). specialize (IN0 (tt, (m0, rv))). fold_eutt. des_ifs.
+    rewrite IN0 in *.
+    eexists _, (SimMemId.mk m0 m0). esplits; et.
+    { econs; et. }
+    left.
+    pfold.
+    econs 1; eauto. clear SUSTAR.
+    ii. clear SU.
+    econs 1; et; swap 2 3.
+    { esplits; intro T; rr in T; des; inv T; ss; rewrite <- IN in *; ss.
+      - rewrite <- IN1 in VIS1. rewrite <- IN0 in VIS1. rewrite interp_trigger in VIS1.
+        cbn in VIS1. rewrite mrec_as_interp in VIS1.
+        cbn in VIS1. des_ifs.
+        cbn in VIS1. autorewrite with itree in VIS1.
+        cbn in VIS1. rewrite bind_trigger in VIS1. vvt VIS1.
+      - rewrite <- IN1 in RET. rewrite <- IN0 in RET. rewrite interp_trigger in RET.
+        cbn in RET. rewrite mrec_as_interp in RET.
+        cbn in RET. des_ifs.
+        cbn in RET. autorewrite with itree in RET.
+        cbn in RET. rewrite bind_trigger in RET. vvt RET.
+    }
+    { eapply modsem_receptive; et. }
+    ii. ss. inv STEPSRC; ss; swap 3 4.
+    { rewrite <- IN in VIS1. rewrite <- IN1 in VIS1. rewrite <- IN0 in VIS1.
+      cbn in VIS1. autorewrite with itree in VIS1.
+      cbn in VIS1. rewrite mrec_as_interp in VIS1.
+      cbn in VIS1. des_ifs.
+      cbn in VIS1. autorewrite with itree in VIS1.
+      cbn in VIS1. rewrite bind_trigger in VIS1. vvt VIS1. }
+    { rewrite <- IN in VIS1. rewrite <- IN1 in VIS1. rewrite <- IN0 in VIS1.
+      cbn in VIS1. autorewrite with itree in VIS1.
+      cbn in VIS1. rewrite mrec_as_interp in VIS1.
+      cbn in VIS1. des_ifs.
+      cbn in VIS1. autorewrite with itree in VIS1.
+      cbn in VIS1. rewrite bind_trigger in VIS1. vvt VIS1. }
+    { rewrite <- IN in VIS1. rewrite <- IN1 in VIS1. rewrite <- IN0 in VIS1.
+      cbn in VIS1. autorewrite with itree in VIS1.
+      cbn in VIS1. rewrite mrec_as_interp in VIS1.
+      cbn in VIS1. des_ifs.
+      cbn in VIS1. autorewrite with itree in VIS1.
+      cbn in VIS1. rewrite bind_trigger in VIS1. vvt VIS1. }
+    hexploit symb; et. i; des.
+    eexists _, _, (SimMemId.mk _ _). esplits; eauto.
+    { left.
+      eapply spread_dplus; et.
+      { eapply modsem2_mi_determinate; et. }
+      eapply plus_left with (t1 := E0) (t2 := E0); ss.
+      { repeat (econs; ss; et); ii; repeat (des; ss; clarify). }
+      eapply star_left with (t1 := E0) (t2 := E0); ss.
+      { repeat (econs; ss; et); ii; repeat (des; ss; clarify). }
+      eapply star_left with (t1 := E0) (t2 := E0); ss.
+      { econs; ss; et.
+        { econs; ss; et.
+          - repeat (econsr; ss; et).
+          - econs 2; ss; et.
+        }
+        repeat (econs; ss; et); ii; repeat (des; ss; clarify).
+        - destruct _fptr; ss.
+        - admit "---------------------------type".
+      }
+      apply star_refl.
+    }
+    right. eapply CIH. econs; ss; et. econs; ss; et.
+    {
+    { rewrite VIS in IN. autorewrite with itree in IN. cbn in IN. rewrite bind_trigger in IN.
+      vvt IN. }
+    { rewrite VIS in IN. autorewrite with itree in IN. cbn in IN. rewrite bind_trigger in IN.
+      vvt IN. }
+    { }
+    eapply CIH. econs; ss; et. econs; et.
+
+      destruct vs; ss.
+      { unfold triggerUB in V. (*** TODO: use notation instead ***)
+        rewrite interp_vis in V. cbn in V. rewrite bind_trigger in V.
+        econs 1; et; swap 2 3.
+        { esplits; intro T; rr in T; des; inv T; ss; rewrite V in *; ss.
+          - vvt VIS.
+          - apply vis_not_ret in RET. ss.
+        }
+        { eapply modsem_receptive; et. }
+        ii. ss. inv STEPSRC; rewrite V in *; try (vvt VIS).
+      }
+      econs 1; eauto; swap 2 3.
+      { esplits; intro T; rr in T; des; inv T; ss. rewrite RET in *.
+        des_ifs;
+          try (by unfold triggerUB, triggerDone in *; autorewrite with itree in V; cbn in V;
+               rewrite bind_trigger in V; sym in V; eapply vis_not_ret in V; ss).
+      }
+      { eapply modsem_receptive; et. }
+      ii. ss. des_ifs.
+      inv STEPSRC.
+
+      rewrite mrec_as_interp in V.
+      rewrite itree_eta_ in V. ss. des_itr itr0; ss. rename V0 into V.
+      rewrite <- itree_eta_ in V. symmetry in V.
+
+      econs 2; try refl; eauto.
+      { esplits; et; cycle 1.
+        { apply Ord.lift_idx_spec. instantiate (1 := Nat.pred idx). xomega. }
+        eapply star_left with (t1 := E0) (t2 := E0); ss.
+        { econs; et. }
+        eapply star_left with (t1 := E0) (t2 := E0); ss.
+        { econs; et. }
+        ss. unfold interp_program0. ss.
+        rewrite itree_eta'. f_equal.
+        unfold interp_OwnedHeapE, interp_MemE, interp_LocalE, interp_GlobalE, ITree.map.
+        unfold interp_state.
+        }
+        econs; eauto.
+      }
+
+      rewrite itree_eta_ in V. ss. des_itr itr0; ss. rename V0 into V.
+      rewrite <- itree_eta_ in V. symmetry in V.
+
+      unfold interp_program0 in V. ss.
+      apply eq_eutt in V.
+      unfold interp_OwnedHeapE, interp_MemE, interp_LocalE, interp_GlobalE, ITree.map in V.
+      rewrite mrec_as_interp in V. ss.
+      autorewrite with itree in V. cbn in V.
+      rewrite interp_state_trigger in V.
+      
+      unfold interp_state.
+      rewrite itree_eta_ in V. ss. des_itr itr0; ss. rewrite <- itree_eta_ in V. symmetry in V.
+      rewrite itree_eta_ in V. ss. des_itr t; ss.
+      { rewrite itree_eta_ in V. unfold observe in V. ss. }
+      rewrite <- itree_eta_ in V.
+      rewrite itree_eta_ in I. ss. des_itr itr0; ss.
+      rewrite itree_eta_ in I. ss.
+      exploit SAFESRC. { apply star_refl. } intro U; des; ss.
+      { rr in EVCALL. des. ss. inv EVCALL. ss.
+        rewrite itree_eta_ in VIS at 1. ss.
+      }
+      { rr in EVRET. des. ss. inv EVRET. ss.
+        rewrite itree_eta_ in RET at 1. ss.
+      }
+      inv EVSTEP; ss. clarify.
+
+      exploit SAFESRC. { apply star_one. econs; eauto. } intro U; des; ss.
+      { rr in EVCALL. des. ss. inv EVCALL. ss.
+        sym in VIS. apply simpobs in VIS. apply bisimulation_is_eq in VIS.
+        clarify.
+      }
+
+      econs 2; try refl; eauto.
+      { esplits; et; cycle 1.
+        { apply Ord.lift_idx_spec. instantiate (1 := Nat.pred idx). xomega. }
+        eapply star_left with (t1 := E0) (t2 := E0); ss.
+        { econs; et. }
+        eapply star_left with (t1 := E0) (t2 := E0); ss.
+        { econs; et. }
+        ss. unfold interp_program0. ss.
+        rewrite itree_eta'. f_equal.
+        unfold interp_OwnedHeapE, interp_MemE, interp_LocalE, interp_GlobalE, ITree.map.
+        unfold interp_state.
+        }
+        econs; eauto.
+      }
+  - econs 1; eauto. ii. clear SU.
+    exploit unsymb; et. intro T. des; clarify.
+    exploit symb_def; et. intro DEF; des. ss. des_ifs.
+    +
+      econs 1; eauto; swap 2 3.
+      { esplits; intro T; rr in T; des; inv T; ss. }
+      { eapply modsem_receptive; et. }
+      ii. ss. inv STEPSRC; ss; clarify; try rewrite TAU in *; clarify.
+      unfold interp_program0 in *. ss.
+
+
+
+      sym in TAU. apply simpobs in TAU. apply eq_sub_eutt in TAU.
+      unfold interp_OwnedHeapE, interp_MemE, interp_LocalE, interp_GlobalE, ITree.map in TAU.
+      
+
+
+
+      (* set (LocalE +' stateE Mem.mem' +' stateE owned_heap +' *)
+      (*        ExternalCallE owned_heap +' DoneE owned_heap +' EventE) as E in *. *)
+      (* { *)
+      (*   rewrite mrec_as_interp in TAU. ss. *)
+      (*   rewrite interp_state_bind in TAU. *)
+      (*   rewrite interp_state_bind in TAU. *)
+      (*   autorewrite with itree in TAU. *)
+      (*   setoid_rewrite interp_bind in TAU. *)
+      (* } *)
+      esplits; et; try refl.
+      { right. esplits; try apply star_refl; eauto.
+        apply Ord.lift_idx_spec. instantiate (1 := Nat.pred idx). xomega.
+      }
+
+
+
+
+
+
+
+
+
+
+      (** need to get some informatino about itr1 *)
+      set (mrec (interp_function IterSource.prog) (ICall _iter vs)) as itr0 in *.
+      destruct (observe itr0) eqn:T; sym in T; apply simpobs in T; apply bisimulation_is_eq in T.
+      { rewrite T in *.
+        autorewrite with itree in TAU.
+        rewrite interp_state_ret in TAU.
+        autorewrite with itree in TAU.
+        rewrite interp_state_ret in TAU.
+        rewrite interp_state_ret in TAU. ss.
+        subst itr0.
+        apply eq_eutt in T.
+        rewrite mrec_as_interp in T. ss.
+        autorewrite with itree in T. ss.
+        rewrite bind_trigger in T. ss.
+        exfalso. eapply vis_not_ret; eauto.
+      }
+      {
+        rewrite T in *.
+        rewrite interp_tau in TAU.
+        rewrite interp_state_tau in TAU.
+        autorewrite with itree in TAU.
+        rewrite interp_state_tau in TAU.
+        rewrite interp_state_tau in TAU.
+        rewrite tau_eutt in TAU.
+        rewrite tau_eutt in TAU.
+
+
+
+
+
+        rewrite bind_tau in TAU.
+        autorewrite with itree in TAU.
+        subst itr0.
+        eapply U in T.
+        rewrite mrec_as_interp in T. ss.
+        rewrite interp_bind in T.
+        rewrite interp_trigger in T. ss.
+        rewrite bind_trigger in T.
+        rewrite interp_interp in T.
+      }
+      { rewrite T in *.
+        rewrite interp_vis in TAU.
+        rewrite interp_state_bind in TAU.
+        rewrite interp_state_bind in TAU.
+        rewrite interp_state_bind in TAU.
+        rewrite interp_state_bind in TAU.
+        rewrite interp_state_bind in TAU.
+        rewrite bind_bind in TAU.
+        unfold interp_state in *.
+        rewrite interp_interp in TAU.
+        rewrite interp_state_ret in TAU.
+        rewrite bind_ret_l in TAU.
+        rewrite interp_state_ret in TAU.
+        rewrite interp_state_ret in TAU. ss.
+        rewrite tau_eutt in TAU.
+        subst itr0.
+        assert(U: forall E R (a b: itree E R), a = b -> eutt eq a b).
+        { i. clarify. refl. }
+        apply U in T.
+        rewrite mrec_as_interp in T. ss.
+        rewrite interp_bind in T.
+        rewrite interp_trigger in T. ss.
+        rewrite bind_trigger in T.
+        exfalso. clear - T.
+        assert(V: forall E R (r: R) X (e: E X) k, Vis e k ≈ Ret r -> False).
+        { clear - vs. clear vs.
+          ii. punfold H. inv H.
+        }
+        eauto.
+      }
+
+
+
+
+
+      left. pfold.
+      ii. clear SUSTAR. econs 1; eauto. ii. clear SU.
+      econs 1; eauto; swap 2 3.
+      { esplits; intro T; rr in T; des; inv T; ss. }
+      { eapply modsem_receptive; et. }
+
+
+
+
+
+
+
+
+
+
+
+
+
+      destruct (observe itr0) eqn:T; sym in T; apply simpobs in T; apply bisimulation_is_eq in T.
+      { rewrite T in *.
+        rewrite interp_ret in TAU.
+        rewrite interp_state_ret in TAU.
+        rewrite bind_ret_l in TAU.
+        rewrite interp_state_ret in TAU.
+        rewrite interp_state_ret in TAU. ss.
+        rewrite tau_eutt in TAU.
+        subst itr0.
+        apply U in T.
+        rewrite mrec_as_interp in T. ss.
+        rewrite interp_bind in T.
+        rewrite interp_trigger in T. ss.
+        rewrite bind_trigger in T.
+        exfalso. eauto.
+      }
+      {
+        rewrite T in *.
+        subst itr0.
+        eapply U in T.
+        rewrite mrec_as_interp in T. ss.
+        rewrite interp_bind in T.
+        rewrite interp_trigger in T. ss.
+        rewrite bind_trigger in T.
+        rewrite interp_interp in T.
+      }
+      { rewrite T in *.
+        rewrite interp_vis in TAU.
+        rewrite interp_state_bind in TAU.
+        rewrite interp_state_bind in TAU.
+        rewrite interp_state_bind in TAU.
+        rewrite interp_state_bind in TAU.
+        rewrite interp_state_bind in TAU.
+        rewrite bind_bind in TAU.
+        unfold interp_state in *.
+        rewrite interp_interp in TAU.
+        rewrite interp_state_ret in TAU.
+        rewrite bind_ret_l in TAU.
+        rewrite interp_state_ret in TAU.
+        rewrite interp_state_ret in TAU. ss.
+        rewrite tau_eutt in TAU.
+        subst itr0.
+        assert(U: forall E R (a b: itree E R), a = b -> eutt eq a b).
+        { i. clarify. refl. }
+        apply U in T.
+        rewrite mrec_as_interp in T. ss.
+        rewrite interp_bind in T.
+        rewrite interp_trigger in T. ss.
+        rewrite bind_trigger in T.
+        exfalso. clear - T.
+        assert(V: forall E R (r: R) X (e: E X) k, Vis e k ≈ Ret r -> False).
+        { clear - vs. clear vs.
+          ii. punfold H. inv H.
+        }
+        eauto.
+      }
+      { rewrite T in *.
+      }
+      rewrite interp_state_bind in TAU.
+      rewrite interp_state_bind in TAU.
+      setoid_rewrite unfold_interp_state in TAU.
+      rewrite mrec_as_interp in TAU. ss.
+      repeat (try rewrite interp_bind in TAU; try setoid_rewrite interp_bind in TAU).
+      setoid_rewrite interp_bind in TAU.
+      setoid_rewrite interp_bind in TAU.
+      rewrite interp_mrecursive.
+      rewrite interp_mrec in *.
+
+mrec_as_interp :
+forall (D E : Type -> Type) (ctx : forall T : Type, D T -> itree (D +' E) T) (T : Type) (d : D T),
+(mrec ctx d ≈ interp (mrecursive ctx) (ctx T d))%itree
+interp_mrecursive :
+forall (D E : Type -> Type) (ctx : forall T : Type, D T -> itree (D +' E) T) (T : Type) (d : D T),
+(interp (mrecursive ctx) (trigger_inl1 d) ≈ mrec ctx d)%itree
+
+
+itree_eta: forall (E : Type -> Type) (R : Type) (t : itree E R), t ≅ {| _observe := observe t |}
+itree_eta':
+  forall (E : Type -> Type) (R : Type) (ot : itree' E R), ot = observe {| _observe := ot |}
+simpobs:
+  forall (E : Type -> Type) (R : Type) (ot : itree' E R) (t : itree E R),
+  ot = observe t -> t ≅ {| _observe := ot |}
+unfold_interp:
+  forall (E F : Type -> Type) (R : Type) (f : forall T : Type, E T -> itree F T) (t : itree E R),
+  interp f t ≅ _interp f (observe t)
+unfold_interp_state:
+  forall (E F : Type -> Type) (S R : Type) (h : forall T : Type, E T -> stateT S (itree F) T)
+    (t : itree E R) (s : S), interp_state h t s ≅ _interp_state h (observe t) s
+
+
+      unfold interp_function in *. ss.
+      rewrite unfold_interp_state in *.
+      esplits; et; try refl.
+      * left. eapply spread_dplus. { eapply modsem2_mi_determinate; et. } eapply plus_one.
+        econs; eauto.
+        { repeat (econs; ss; eauto; ii; ss; des; clarify).
+      left.
+  -
+Qed.
+
