demo/fib/FibSource.v
@@ -1,0 +1,49 @@
+Require Import CoqlibC Maps.
+Require Import ASTC Integers ValuesC EventsC MemoryC Globalenvs.
+Require Import Op Registers.
+Require Import sflib.
+Require Import SmallstepC.
+Require Export Simulation.
+Require Import Skeleton Mod ModSem.
+Require ClightC.
+Require Import FibTarget.
+Require Import SIRmini_quotient.
+(* Require Import Clightdefs. *)
+
+Set Implicit Arguments.
+
+
+
+Definition owned_heap: Type := unit.
+Definition initial_owned_heap: SkEnv.t -> owned_heap := fun _ => tt.
+
+Definition c_fib (oh0: owned_heap) (m0: mem) (vs: list val):
+  itree (E owned_heap) (owned_heap * (mem * val)) :=
+  match vs with
+  | [Vint n] =>
+    if Int.eq n Int.zero
+    then Ret (oh0, (m0, (Vint Int.zero)))
+    else
+      if Int.eq n Int.one
+      then Ret (oh0, (m0, (Vint Int.one)))
+      else
+        '(oh1, (m1, y1)) <- trigger (ICall _fib oh0 m0 [Vint (Int.sub n (Int.repr 2))]) ;;
+        '(oh2, (m2, y2)) <- trigger (ICall _fib oh0 m0 [Vint (Int.sub n (Int.repr 1))]) ;;
+        Ret (oh2, (m2, Val.add y1 y2))
+  | _ => triggerUB (owned_heap := owned_heap)
+  end
+.
+
+Definition f_fib: function owned_heap :=
+  mkfunction (ClightC.signature_of_function f_fib)
+             (fun oh0 m0 vs => trigger (EBP _) ;; c_fib oh0 m0 vs).
+
+Definition global_definitions: list (ident * globdef (fundef (function owned_heap)) unit) :=
+((_fib, Gfun(Internal f_fib)) ::
+ nil
+)
+.
+
+Definition prog: program owned_heap := mkprogram global_definitions public_idents _main.
+
+Definition module: Mod.t := module prog "fib"%string initial_owned_heap.
