demo/fib/FibTarget.v
@@ -1,0 +1,63 @@
+From Coq Require Import String List ZArith.
+From compcert Require Import Coqlib Integers Floats AST Ctypes Cop Clight Clightdefs.
+Local Open Scope Z_scope.
+
+Definition _fib : ident := 56%positive.
+Definition _main : ident := 57%positive.
+Definition _n : ident := 53%positive.
+Definition _y1 : ident := 54%positive.
+Definition _y2 : ident := 55%positive.
+Definition _t'1 : ident := 58%positive.
+Definition _t'2 : ident := 59%positive.
+
+Definition f_fib := {|
+  fn_return := tint;
+  fn_callconv := cc_default;
+  fn_params := ((_n, tint) :: nil);
+  fn_vars := nil;
+  fn_temps := ((_y1, tint) :: (_y2, tint) :: (_t'2, tint) :: (_t'1, tint) ::
+               nil);
+  fn_body :=
+(Ssequence
+  (Sifthenelse (Ebinop Oeq (Etempvar _n tint) (Econst_int (Int.repr 0) tint)
+                 tint)
+    (Sreturn (Some (Econst_int (Int.repr 0) tint)))
+    Sskip)
+  (Ssequence
+    (Sifthenelse (Ebinop Oeq (Etempvar _n tint)
+                   (Econst_int (Int.repr 1) tint) tint)
+      (Sreturn (Some (Econst_int (Int.repr 1) tint)))
+      Sskip)
+    (Ssequence
+      (Ssequence
+        (Scall (Some _t'1)
+          (Evar _fib (Tfunction (Tcons tint Tnil) tint cc_default))
+          ((Ebinop Osub (Etempvar _n tint) (Econst_int (Int.repr 1) tint)
+             tint) :: nil))
+        (Sset _y1 (Etempvar _t'1 tint)))
+      (Ssequence
+        (Ssequence
+          (Scall (Some _t'2)
+            (Evar _fib (Tfunction (Tcons tint Tnil) tint cc_default))
+            ((Ebinop Osub (Etempvar _n tint) (Econst_int (Int.repr 2) tint)
+               tint) :: nil))
+          (Sset _y2 (Etempvar _t'2 tint)))
+        (Sreturn (Some (Ebinop Oadd (Etempvar _y1 tint) (Etempvar _y2 tint)
+                         tint)))))))
+|}.
+
+Definition composites : list composite_definition :=
+nil.
+
+Definition global_definitions : list (ident * globdef fundef type) :=
+((_fib, Gfun(Internal f_fib)) :: nil).
+
+Definition public_idents : list ident :=
+(_fib :: nil).
+
+Definition prog : Clight.program := 
+  mkprogram composites global_definitions public_idents _main Logic.I.
+
+Require Import Mod ClightC.
+
+Definition module: Mod.t := module2_mi prog (Some "fib"%string).
